Azurite/UInt64/Equiv/Basic.lean
@@ -1,0 +1,6 @@
+import Mathlib.Data.UInt
+
+/-- `UInt64` values are equal iff their `toNat` images are equal. -/
+lemma UInt64.eq_of_toNat_eq {x y : UInt64} (h : x.toNat = y.toNat) : x = y := by
+  have h2 : x.toBitVec = y.toBitVec := BitVec.eq_of_toNat_eq h
+  cases x; cases y; simp at h2; subst h2; rfl
